Rfc4648.lean
@@ -5,5 +5,4 @@ import Rfc4648.Alphabet
 import Rfc4648.Base16
 import Rfc4648.Base32
 import Rfc4648.Base64
-import Rfc4648.Fast
 import Rfc4648.Length
